Revised build so that system can be separately compiled. Also moved test programs to separate directory.

examples/dev/sw2/Normal.sig
@@ -1,0 +1,17 @@
+signature Normal = 
+sig
+  include Abbrev
+
+  val PRE_PROCESS_RULE : thm -> thm
+  val SUBST_2_RULE : thm * thm -> thm -> thm
+  val Normalize_Atom_Cond : thm * thm * thm * thm -> conv
+  val K_Normalize : conv
+  val normalize : thm -> thm
+  val identify_atom : term -> term
+  val beta_reduction : thm -> thm
+  val ELIM_LET_RULE : thm -> thm
+  val FLATTEN_LET_RULE : thm -> thm
+  val to_ssa : string -> term -> term
+  val SSA_CONV : conv
+  val SSA_RULE : thm -> thm
+end
