examples/dev/sw2/SALGen.sig
@@ -1,0 +1,6 @@
+signature SALGen =
+sig
+ include Abbrev
+ val forward_reason : term -> thm
+ val certified_gen : thm -> thm
+end
