examples/dev/sw2/basic.sig
@@ -1,0 +1,13 @@
+signature basic =
+sig
+  include Abbrev
+  val is_word_literal : term -> bool
+  val is_atom : term -> bool 
+  val is_binop : term -> bool 
+  val is_cmpop : term -> bool 
+  val is_relop : term -> bool 
+  val is_atom_cond : term -> bool 
+  val subst_exp : (term,term) subst -> term -> term
+  val occurs_in : term -> term -> bool 
+  val abs_fun : thm -> thm
+end
