examples/dev/sw2/inline.sig
@@ -1,0 +1,15 @@
+signature inline =
+sig
+  include Abbrev
+  val threshold : int ref
+  val unroll_limit : int ref
+
+  val size : term -> int
+  val identify_small_fun : term -> term
+  val once_expand_anonymous : thm -> thm
+  val expand_anonymous : thm -> thm
+  val mk_inline_rules : thm list -> thm list
+  val expand_named : thm list -> thm -> thm
+  val optimize : thm -> thm
+  val optimize_norm : thm list -> thm -> thm
+end
