examples/dev/sw2/regAlloc.sig
@@ -1,0 +1,16 @@
+signature regAlloc =
+sig
+  include Abbrev
+
+  datatype alloc_result 
+     = Alloc of term (* allocated register *)
+     | Spill of term (* spilled variable *)
+
+  val DEBUG : bool ref
+  val allregs : term list
+  val reg_sp : term
+  val reg_hp : term
+  val regL : term list ref
+  val alloc_mem : term -> term
+  val reg_alloc : thm -> thm
+end
