examples/dev/sw2/NormalScript.sml
@@ -1,0 +1,271 @@
+open HolKernel Parse boolLib bossLib;
+
+val _ = new_theory"Normal";
+
+val C_def = Define `
+    C e = \k. k e`;
+
+val atom_def = Define `
+    atom = \x.x`;
+
+val C_ATOM_INTRO = Q.store_thm (
+  "C_ATOM_INTRO",
+  `!v. C v = C (atom v)`,
+  SIMP_TAC std_ss [atom_def, C_def]
+ );
+
+val ATOM_ID = Q.store_thm (
+   "ATOM_ID",
+   `atom x = x`,
+   SIMP_TAC std_ss [atom_def]
+  );
+
+val C_ATOM = Q.store_thm (
+  "C_ATOM",
+  `C (atom v) =
+      \k. k v`,
+  SIMP_TAC std_ss [C_def, atom_def]
+ );
+
+val C_INTRO = Q.store_thm (
+  "C_INTRO",
+  `!f. f = C f (\x.x)`,
+  SIMP_TAC std_ss [C_def, LET_THM]
+ );
+
+val C_2_LET = Q.store_thm (
+  "C_2_LET",
+  `(C e k = let x = e in k x)`,
+  SIMP_TAC std_ss [C_def, atom_def, LET_THM]
+ );
+
+(*---------------------------------------------------------------------------*)
+(* Convert an expression to it continuation format                           *)
+(* Theorems used for rewriting                                               *)	
+(*---------------------------------------------------------------------------*)
+
+val C_BINOP = Q.store_thm (
+  "C_BINOP",
+   `(C (e1 + e2) = \k. C e1 (\x. C e2 (\y. C (x + y) k))) /\
+    (C (e1 - e2) = \k. C e1 (\x. C e2 (\y. C (x - y) k))) /\
+    (C (e1 * e2) = \k. C e1 (\x. C e2 (\y. C (x * y) k))) /\
+    (C (e1 ** e2) = \k. C e1 (\x. C e2 (\y. C (x ** y) k)))`,
+   SIMP_TAC std_ss [C_def, LET_THM]
+  );
+
+val C_PAIR = Q.store_thm (
+  "C_PAIR",
+  `C (e1, e2) = \k. C e1 (\x. C e2 (\y. k (x,y)))`,
+   SIMP_TAC std_ss [C_def, LET_THM]
+  );
+
+(*  LET expressions are processed in a way that generate A-normal forms *)
+
+val C_LET = Q.store_thm (
+  "C_LET",
+  `C (let v = e in f v) = \k. C e (\x. C (f x) (\y. k y))`,
+   SIMP_TAC std_ss [C_def, LET_THM]
+  );
+
+(*  For K-normal forms, use the following for LET expressions *)
+
+val C_LET_K = Q.store_thm (
+  "C_LET_K",
+   `C (let v = e in f v) = \k. C e (\x. C x (\y. C (f y) (\z.k z)))`,
+   SIMP_TAC std_ss [C_def, LET_THM]
+  );
+
+val C_ABS = Q.store_thm (
+  "C_ABS",
+   `C (\v. f v) = C (\v. (C (f v) (\x. x)))`,
+   RW_TAC std_ss [C_def, LET_THM]
+  );
+
+val C_APP = Q.store_thm (
+  "C_APP",
+   `C (f e) = \k. C f (\g. C e (\x. C (g x) (\y. k y)))`,
+   SIMP_TAC std_ss [C_def, LET_THM]
+  );
+
+val C_ATOM_COND = Q.store_thm (
+  "C_ATOM_COND",
+   `C (if cmpop c1 c2 then e1 else e2) = 
+       \k. C c1 (\p. C c2 (\q.
+         C (if cmpop p q then C e1 (\x.x) 
+            else C e2 (\y.y)) (\z. k z)))`,
+   SIMP_TAC std_ss [C_def, LET_THM]
+  );
+
+(*
+val C_COMPOUND_COND = Q.store_thm (
+  "C_COMPOUND_COND",
+   `C (if c1 /\ c2 then e1 else e2) = 
+       \k. C c1 (\p. C c2 (\q. C e1 (\x. C e2 
+           (\y. k (if p then 
+                   if q then x else y
+                   else y)))))`,
+   RW_TAC std_ss [C_def, LET_THM] THEN
+   METIS_TAC []
+  );
+*)
+
+
+val BETA_REDUCTION = Q.store_thm (
+   "BETA_REDUCTION",
+   `(let x = atom y in f x) = f y`,
+   SIMP_TAC std_ss [atom_def, LET_THM]
+  );
+
+val ELIM_USELESS_LET = Q.store_thm (
+  "ELIM_USELESS_LET",
+   `(let x = e1 in e2) = e2`,
+   SIMP_TAC std_ss [C_def, LET_THM]
+  );
+
+val FLATTEN_LET = Q.store_thm (
+  "FLATTEN_LET",
+   `(let x = (let y = e1 in e2 y) in e3 x) = (let y = e1 in let x = e2 y in e3 x)`,
+   SIMP_TAC std_ss [LET_THM]
+  );
+
+
+(* Conjunction in condtions *)
+val AND_COND = Q.store_thm (
+  "AND_COND",
+  `(if c1 /\ c2 then e1 else e2) = 
+     let x = e2 in
+      (if c1 then 
+         if c2 then e1 else x
+       else x)`,
+   RW_TAC std_ss [LET_THM] THEN
+   METIS_TAC []
+  );
+
+(* Disjunction in condtions *)
+val OR_COND = Q.store_thm (
+  "OR_COND",
+  `(if c1 \/ c2 then e1 else e2) = 
+    let x = e1 in
+      (if c1 then x else
+       if c2 then x else e2)`,
+   RW_TAC std_ss [LET_THM] THEN
+   METIS_TAC []
+  );
+
+(* Normalize the conditions in branches *)
+val BRANCH_NORM = Q.store_thm (
+  "BRANCH_NORM",
+  `((if a > b then x else y) = (if a <= b then y else x)) /\ 
+    ((if a >= b then x else y) = (if b <= a then x else y)) /\
+    ((if a < b then x else y) = (if b <= a then y else x))
+  `,
+   RW_TAC arith_ss [] THEN
+   FULL_SIMP_TAC std_ss [arithmeticTheory.GREATER_DEF, arithmeticTheory.GREATER_EQ,
+          arithmeticTheory.NOT_LESS, arithmeticTheory.NOT_LESS_EQUAL] THEN
+   METIS_TAC [arithmeticTheory.LESS_EQ_ANTISYM]
+  );
+
+
+(*---------------------------------------------------------------------------*)
+(* Definitions used in inline.sml                                            *)
+(*---------------------------------------------------------------------------*)
+
+val fun_def = Define `
+  fun = \x.x`;
+
+val fun_ID = store_thm (
+  "fun_ID",
+  ``fun f = f``,
+   SIMP_TAC std_ss [fun_def]
+  );
+
+val INLINE_EXPAND = store_thm (
+  "INLINE_EXPAND",
+  ``(let f = fun e1 in e2 f) = e2 e1``,
+   SIMP_TAC std_ss [LET_THM, fun_def]
+  );
+
+
+(* Definitions and theorems used in closure.sml *)
+(*---------------------------------------------------------------------------*)
+(* Closure conversion                                                        *)
+(* Eliminate nested function definitions                                     *)
+(*---------------------------------------------------------------------------*)
+
+val CLOSE_ONE = store_thm (
+  "CLOSE_ONE",
+  ``(let v = atom v in let f = fun (e1 v) in e2 f) = 
+    let f = fun (\v. e1 v) in e2 (f v)``,
+   SIMP_TAC std_ss [LET_THM, fun_def, atom_def]
+  );
+
+(*---------------------------------------------------------------------------*)
+(* Eliminate administrative terms                                            *)
+(*---------------------------------------------------------------------------*)
+
+val LET_ATOM = store_thm (
+  "LET_ATOM",
+  ``(let x = atom x in f x) = f x``,
+   SIMP_TAC std_ss [LET_THM, atom_def]
+  );
+
+val LET_FUN = store_thm (
+  "LET_FUN",
+  ``(let f = fun e1 in e2 f) = e2 e1``,
+   SIMP_TAC std_ss [LET_THM, fun_def]
+  );
+
+
+val TOP_LEVEL_ABS = store_thm (
+  "TOP_LEVEL",
+  ``(\x. let f = fun e1 in e2 f) = (let f = fun e1 in (\x. e2 f))``,
+   SIMP_TAC std_ss [LET_THM]
+  );
+
+val TOP_LEVEL_LET = store_thm (
+  "TOP_LEVEL_LET",
+  ``(let v = e1 in let f = fun e2 in e3 v f) = 
+    (let f = fun e2 in let v = e1 in e3 v f)``,
+   SIMP_TAC std_ss [LET_THM]
+  );
+
+val TOP_LEVEL_COND_1 = store_thm (
+  "TOP_LEVEL_COND_1",
+  ``(if e1 then let f = fun k1 in e2 f else e3) = 
+        (let f = fun k1 in if e1 then e2 f else e3)``,
+   SIMP_TAC std_ss [LET_THM]
+  );
+
+val TOP_LEVEL_COND_2 = store_thm (
+  "TOP_LEVEL_COND_2",
+  ``(if e1 then e2 else let f = fun k1 in e3 f) =
+        (let f = fun k1 in if e1 then e2 else e3 f)``,
+   SIMP_TAC std_ss [LET_THM]
+  );
+
+
+(* --------------------------------------------------------------------*)
+(* Used in regAlloc.sml                                                *)
+(* Administrative terms: save and loc                                  *)
+(* --------------------------------------------------------------------*)
+
+val save_def = Define `
+  save = \x.x`;
+
+val LET_SAVE = store_thm (
+  "LET_SAVE",
+  ``(let x = save y in f x) = f y``,
+   SIMP_TAC std_ss [LET_THM, save_def]
+  );
+
+val loc_def = Define `
+  loc = \x.x`;
+
+val LET_LOC = store_thm (
+  "LET_LOC",
+  ``(let x = loc y in f x) = f y``,
+   SIMP_TAC std_ss [LET_THM, loc_def]
+  );
+
+
+val _ = export_theory();
