examples/dev/sw2/closure.sml
@@ -1,31 +1,11 @@
+structure closure :> closure =
+struct
 
-(*---------------------------------------------------------------------------*)
-(* Closure conversion                                                        *)
-(* Eliminate nested function definitions                                     *)
-(*---------------------------------------------------------------------------*)
+open HolKernel Parse boolLib pairLib PairRules simpLib boolSimps bossLib
+     NormalTheory pairSyntax basic Normal;
 
-val CLOSE_ONE = store_thm (
-  "CLOSE_ONE",
-  ``(let v = atom v in let f = fun (e1 v) in e2 f) = 
-    let f = fun (\v. e1 v) in e2 (f v)``,
-   SIMP_TAC std_ss [LET_THM, fun_def, atom_def]
-  );
-
-(*---------------------------------------------------------------------------*)
-(* Eliminate administrative terms                                            *)
-(*---------------------------------------------------------------------------*)
-
-val LET_ATOM = store_thm (
-  "LET_ATOM",
-  ``(let x = atom x in f x) = f x``,
-   SIMP_TAC std_ss [LET_THM, atom_def]
-  );
-
-val LET_FUN = store_thm (
-  "LET_FUN",
-  ``(let f = fun e1 in e2 f) = e2 e1``,
-   SIMP_TAC std_ss [LET_THM, fun_def]
-  );
+val atom_tm = prim_mk_const{Name="atom",Thy="Normal"};
+val fun_tm = prim_mk_const{Name="fun",Thy="Normal"};
 
 (*---------------------------------------------------------------------------*)
 (* Close the function variable by variable                                   *)
@@ -33,14 +13,16 @@ val LET_FUN = store_thm (
 (*---------------------------------------------------------------------------*)
 
 fun abs_fvars tm = 
-  let 
-     fun close_up f body = 
-       List.foldl (fn (v,t) => mk_plet (v, mk_comb (inst [alpha |-> type_of v] ``atom``, v), t)) f (free_vars body)
+ let fun close_up f body = 
+      List.foldl 
+       (fn (v,t) => mk_plet(v,mk_comb(inst[alpha |-> type_of v] atom_tm,v),t)) 
+       f (free_vars body)
      fun trav t = 
        if is_let t then 
            let val (v,M,N) = dest_plet t in
                if is_pabs M then 
-                 close_up (mk_plet (v, mk_comb (inst [alpha |-> type_of M] ``fun``, trav M), trav N)) M 
+                 close_up (mk_plet 
+                     (v, mk_comb(inst[alpha |-> type_of M] fun_tm,trav M),trav N)) M 
                else mk_plet (v, trav M, trav N)
            end
        else if is_cond t then
@@ -79,7 +61,7 @@ fun identify_fun tm =
        if is_let t then 
            let val (v,M,N) = dest_plet t in
                if is_pabs M then 
-                 mk_plet (v, mk_comb (inst [alpha |-> type_of M] ``fun``, trav M), trav N) 
+                 mk_plet (v, mk_comb (inst [alpha |-> type_of M] fun_tm, trav M), trav N) 
                else mk_plet (v, trav M, trav N)
            end
        else if is_cond t then
@@ -105,7 +87,7 @@ fun abs_all_fvars tm =
                       val (M',N') = (trav M, trav N)
                       val f = mk_pabs (cls, M')
                       val v' = (mk_var (term_to_string v, type_of f))
-                      val f' = mk_comb (inst [alpha |-> type_of f] ``fun``, f)
+                      val f' = mk_comb (inst [alpha |-> type_of f] fun_tm, f)
                       val N'' = subst_exp [v |-> mk_comb (v', cls)] N'
                   in
                      mk_plet (v', f', N'')
@@ -143,35 +125,8 @@ fun close_all def =
 (*   Move all functions definitions to top level                             *)  
 (*---------------------------------------------------------------------------*)
 
-val TOP_LEVEL_ABS = store_thm (
-  "TOP_LEVEL",
-  ``(\x. let f = fun e1 in e2 f) = (let f = fun e1 in (\x. e2 f))``,
-   SIMP_TAC std_ss [LET_THM]
-  );
-
-val TOP_LEVEL_LET = store_thm (
-  "TOP_LEVEL_LET",
-  ``(let v = e1 in let f = fun e2 in e3 v f) = 
-    (let f = fun e2 in let v = e1 in e3 v f)``,
-   SIMP_TAC std_ss [LET_THM]
-  );
-
-val TOP_LEVEL_COND_1 = store_thm (
-  "TOP_LEVEL_COND_1",
-  ``(if e1 then let f = fun k1 in e2 f else e3) = 
-        (let f = fun k1 in if e1 then e2 f else e3)``,
-   SIMP_TAC std_ss [LET_THM]
-  );
-
-val TOP_LEVEL_COND_2 = store_thm (
-  "TOP_LEVEL_COND_2",
-  ``(if e1 then e2 else let f = fun k1 in e3 f) =
-        (let f = fun k1 in if e1 then e2 else e3 f)``,
-   SIMP_TAC std_ss [LET_THM]
-  );
-
-val TOP_LEVEL_RULE = SIMP_RULE pure_ss [TOP_LEVEL_LET, TOP_LEVEL_COND_1, TOP_LEVEL_COND_2];
- (* may loop forever, to be improved *)
+val TOP_LEVEL_RULE =  (* may loop forever, to be improved *)
+  SIMP_RULE pure_ss [TOP_LEVEL_LET, TOP_LEVEL_COND_1, TOP_LEVEL_COND_2];
 
 (*---------------------------------------------------------------------------*)
 (*   Closure conversion                                                      *)
@@ -187,3 +142,6 @@ fun closure_convert def =
   in
     th4
   end
+
+end (* struct *)
+
